src/ReactorModel/Execution/State.lean
@@ -3,39 +3,31 @@ import ReactorModel.Execution.Reactor
 noncomputable section
 open Classical ReactorType 
 
-namespace List
-
-def targets (cs : List Change) :=
-  { t : Component.Valued × ID | ∃ c ∈ cs, c.Targets t.fst t.snd }
-
-theorem mem_targets_cons (h : t ∈ tl.targets) : t ∈ (hd :: tl).targets := by
-  have ⟨c, hm, _⟩ := h 
-  exists c, by simp [hm]
-
-theorem target_mem_targets {cs : List Change} (hc : c ∈ cs) (ht : c.target = some t) : 
-    t ∈ cs.targets := by
-  exists c, hc
-  cases c <;> simp [Change.target] at *
-  subst ht
-  constructor
-
-end List
-
 namespace Execution
-
-@[ext]
-structure State (α) [Indexable α] where
-  rtr      : α 
-  tag      : Time.Tag
-  progress : Set ID
-  events   : ID ⇀ Time.Tag ⇉ Value -- For each action we keep a mapping of tag to value.
 
 variable [Indexable α]
 
+@[ext]
+structure State (α) where
+  rtr      : α 
+  tag      : Time.Tag
+  progress : Set ID
+  events   : ID ⇀ Time.Tag ⇉ Value
+
 namespace State
 
-def actions (s : State α) (g : Time.Tag) : ID ⇀ Value := 
-  fun i => s.events i >>= (· g)
+def input (s : State α) (rcn : ID) : Reaction.Input where
+  val cpt := s.rtr[.rcn][rcn] |>.elim ∅ (restriction · cpt)
+  tag := s.tag
+where 
+  restriction (rcn : Reaction) (cpt : Component.Valued) := 
+    s.rtr[cpt].restrict { i | ⟨cpt, i⟩ ∈ rcn.deps .in }
+
+def output (s : State α) (rcn : ID) : Reaction.Output := 
+  s.rtr[.rcn][rcn] |>.elim [] (· $ s.input rcn)
+
+def record (s : State α) (rcn : ID) : State α := 
+  { s with progress := s.progress.insert rcn }
 
 def schedule (s : State α) (i : ID) (t : Time) (v : Value) : State α := 
   { s with events := s.events.update i (go · t v) }
@@ -48,236 +40,26 @@ where
 def scheduledTags (s : State α) : Set Time.Tag := 
   { g | ∃ i a, (s.events i = some a) ∧ (g ∈ a.keys) }
 
-scoped macro "cases_change " change:term : tactic => `(tactic| 
-  cases $change:term <;> try cases ‹Change.Normal›; cases ‹Component.Valued›
-)
-
-/-
-theorem apply_equiv (s : State α) (c : Change) : (apply s c).rtr ≈ s.rtr := by
-  cases_change c <;> first | exact .refl _ | apply Equivalent.symm; apply LawfulUpdatable.equiv
-
-theorem apply_preserves_tag (s : State α) (c : Change) : (apply s c).tag = s.tag := by
-  cases_change c <;> rfl
-
-theorem apply_preserves_progress (s : State α) (c : Change) : 
-    (apply s c).progress = s.progress := by
-  cases_change c <;> rfl
-
-theorem apply_preserves_unchanged {c : Change} (s : State α) (h : ¬c.Targets cpt i) :
-    (apply s c).rtr[cpt][i] = s.rtr[cpt][i] := by
-  cases_change c
-  all_goals first | exact .refl _ | exact LawfulUpdatable.obj?_preserved (Change.Targets.norm_not h)
-
-variable {s : State α} in section
-
-theorem apply_input_change (h : i ∈ s.rtr[.inp]) : (apply s $ .inp i v).rtr[.inp][i] = some v := by
-  simp [apply, LawfulUpdatable.obj?_updated]
-  exact h
-
-theorem apply_output_change (h : i ∈ s.rtr[.out]) : (apply s $ .out i v).rtr[.out][i] = some v := by
-  simp [apply, LawfulUpdatable.obj?_updated]
-  exact h
-
-theorem apply_state_change (h : i ∈ s.rtr[.stv]) : (apply s $ .stv i v).rtr[.stv][i] = some v := by
-  simp [apply, LawfulUpdatable.obj?_updated]
-  exact h
-
-theorem apply_ne_target_comm (ht : c₁.target ≠ c₂.target ∨ c₁.target = none) : 
-    apply (apply s c₁) c₂ = apply (apply s c₂) c₁ := by
-  ext1 <;> cases_change c₁ <;> cases_change c₂ <;> simp [apply, Change.target] at *
-  all_goals 
-    try rfl
-    try exact LawfulUpdatable.update_ne_comm $ by simp_all
-  apply Partial.update_ne_comm _ ht
-
-theorem apply'_equiv (s : State α) : (cs : List Change) → (apply' s cs).rtr ≈ s.rtr 
-  | .nil        => .refl _
-  | .cons hd tl => Equivalent.trans (apply'_equiv (apply s hd) tl) (apply_equiv s hd)
-
-theorem apply'_preserves_tag (cs : List Change) : (apply' s cs).tag = s.tag := by
-  induction cs generalizing s
-  case nil => rfl
-  case cons hd tl hi => exact apply_preserves_tag s hd ▸ @hi (apply s hd)
-
-theorem apply'_preserves_progress (cs : List Change) : (apply' s cs).progress = s.progress := by
-  induction cs generalizing s
-  case nil => rfl
-  case cons hd tl hi => exact apply_preserves_progress s hd ▸ @hi (apply s hd)
-
-theorem apply'_preserves_unchanged {cs : List Change} {cpt : Component.Valued} {i}
-    (h : cs.All₂ (¬·.Targets cpt i)) : (apply' s cs).rtr[cpt][i] = s.rtr[cpt][i] := by
-  induction cs generalizing s <;> try rfl
-  case cons hd tl hi => 
-    have ⟨hh, ht⟩ := List.all₂_cons _ _ _ |>.mp h
-    exact apply_preserves_unchanged s hh ▸ hi ht 
-
-theorem apply'_apply_ne_targets_comm (ht : ∀ {t}, c.target = some t → t ∉ cs.targets) : 
-    apply (apply' s cs) c = apply' (apply s c) cs := by
-  induction cs generalizing s <;> simp [apply'] at *
-  case cons hd tl hi =>
-    suffices h : hd.target ≠ c.target ∨ hd.target = none by 
-      rw [hi $ fun _ _ h hm => ht _ _ h $ List.mem_targets_cons hm, apply_ne_target_comm h]
-    by_contra hc
-    push_neg at hc
-    have ⟨_, h⟩ := Option.ne_none_iff_exists.mp hc.right
-    exact ht _ _ (hc.left ▸ h.symm) $ List.target_mem_targets (by simp) h.symm
-
-theorem apply'_disjoint_targets_comm (ht : Disjoint cs₁.targets cs₂.targets) : 
-    apply' (apply' s cs₁) cs₂ = apply' (apply' s cs₂) cs₁ := by
-  induction cs₁ generalizing s <;> cases cs₂ <;> simp [apply'] at *
-  case cons.cons hd₁ tl₁ hd₂ tl₂ hi =>
-    have h₁ : Disjoint (List.targets tl₁) (List.targets (hd₂ :: tl₂)) := by
-      simp [Set.disjoint_iff_forall_ne]
-      intro _ _ hm₁ _ _ hm₂ h₁ h₂
-      subst h₁ h₂    
-      exact Set.disjoint_left.mp ht (List.mem_targets_cons hm₁) hm₂
-    have h₂ : hd₁.target ≠ hd₂.target ∨ hd₁.target = none := by
-      by_contra hc
-      push_neg at hc
-      have ⟨_, h⟩ := Option.ne_none_iff_exists.mp hc.right
-      have h₁ := (hd₁ :: tl₁).target_mem_targets (by simp) h.symm
-      have h₂ := (hd₂ :: tl₂).target_mem_targets (by simp) (hc.left ▸ h.symm)
-      exact Set.disjoint_left.mp ht h₁ h₂
-    have h₃ : ∀ {t}, hd₁.target = some t → ¬t ∈ tl₂.targets := by
-      intro _ h hm
-      have h₁ := (hd₁ :: tl₁).target_mem_targets (by simp) h
-      exact Set.disjoint_left.mp ht h₁ $ List.mem_targets_cons hm
-    rw [hi h₁, apply_ne_target_comm h₂, ←apply', ←apply', ←apply'_apply_ne_targets_comm h₃]
-    rfl
-
-end
--/
-
-def Closed (s : State α) : Prop := 
-  s.progress = s.rtr[.rcn].ids
+def actions (s : State α) (g : Time.Tag) : ID ⇀ Value := 
+  fun i => s.events i >>= (· g)
 
 structure Allows (s : State α) (rcn : ID) : Prop where
   mem         : rcn ∈ s.rtr[.rcn] 
   deps        : dependencies s.rtr rcn ⊆ s.progress
   unprocessed : rcn ∉ s.progress
 
-namespace Allows
-
-variable {s : State α}
-
-theorem «def» : 
-    (s.Allows i) ↔ (i ∈ s.rtr[.rcn]) ∧ (dependencies s.rtr i ⊆ s.progress) ∧ (i ∉ s.progress) where
-  mp  := fun ⟨mem, deps, unprocessed⟩ => ⟨mem, deps, unprocessed⟩
-  mpr := fun ⟨mem, deps, unprocessed⟩ => ⟨mem, deps, unprocessed⟩
-
-theorem acyclic (a : s.Allows rcn) : ¬(rcn <[s.rtr] rcn) :=
-  (a.unprocessed $ a.deps ·)
-
-theorem not_elim (a : ¬s.Allows rcn) : 
-    (rcn ∉ s.rtr[.rcn]) ∨ (∃ i, i ∈ dependencies s.rtr rcn ∧ i ∉ s.progress) ∨ (rcn ∈ s.progress) 
-    := by
-  by_contra h
-  push_neg at h
-  exact a { mem := h.left, deps := h.right.left, unprocessed := h.right.right }
-
-end Allows
-
-def input (s : State α) (rcn : ID) : Reaction.Input where
-  val cpt := s.rtr[.rcn][rcn] |>.elim ∅ (restriction · cpt)
-  tag := s.tag
-where 
-  restriction (rcn : Reaction) (cpt : Component.Valued) := 
-    s.rtr[cpt].restrict { i | ⟨cpt, i⟩ ∈ rcn.deps .in }
-
-theorem input_progress_agnostic {s₁ s₂ : State α}
-    (hr : s₁.rtr = s₂.rtr := by rfl) (ht : s₁.tag = s₂.tag := by rfl) : 
-    s₁.input i = s₂.input i := by
-  simp [input, input.restriction, hr, ht]
-
-def output (s : State α) (rcn : ID) : List Change := 
-  s.rtr[.rcn][rcn] |>.elim [] (· $ s.input rcn)
-
-theorem output_progress_agnostic {s₁ s₂ : State α}
-    (hr : s₁.rtr = s₂.rtr := by rfl) (ht : s₁.tag = s₂.tag := by rfl) : 
-    s₁.output i = s₂.output i := by
-  simp [output, input_progress_agnostic hr ht, hr]
-
 inductive Triggers (s : State α) (i : ID) : Prop
-  | intro (mem : s.rtr[.rcn][i] = some rcn) (triggers : rcn.TriggersOn (s.input i))
-
-theorem Triggers.def {s : State α} : 
-    (s.Triggers i) ↔ (∃ rcn, (s.rtr[.rcn][i] = some rcn) ∧ rcn.TriggersOn (s.input i)) where
-  mp  := fun ⟨mem, triggers⟩ => ⟨_, mem, triggers⟩   
-  mpr := fun ⟨_, mem, triggers⟩ => .intro mem triggers
-
-theorem Triggers.progress_agnostic {s₁ s₂ : State α}
-    (hr : s₁.rtr = s₂.rtr := by rfl) (ht : s₁.tag = s₂.tag := by rfl) : 
-    Triggers s₁ i ↔ Triggers s₂ i := by
-  simp [Triggers.def, hr, input_progress_agnostic hr ht]    
-
-def record [DecidableEq ID] (s : State α) (rcn : ID) : State α := 
-  { s with progress := s.progress.insert rcn }
-
-theorem record_comm {s : State α} {rcn₁ rcn₂ : ID} : 
-    (s.record rcn₁).record rcn₂ = (s.record rcn₂).record rcn₁ := by
-  simp [record]
-  apply Set.insert_comm 
-
-theorem record_preserves_rtr (s : State α) (rcn : ID) : (s.record rcn).rtr = s.rtr := 
-  rfl
-
-theorem record_preserves_tag (s : State α) (rcn : ID) : (s.record rcn).tag = s.tag := 
-  rfl
-
-theorem record_preserves_events (s : State α) (rcn : ID) : (s.record rcn).events = s.events := 
-  rfl
-
-theorem record_progress_eq (s : State α) (rcn₁ rcn₂ : ID) : 
-    (s.record rcn).progress = s.progress.insert rcn := 
-  rfl
-
-/- TODO: Delete if unused.
-theorem mem_record_progress_iff (s : State α) (rcn₁ rcn₂ : ID) : 
-    rcn₁ ∈ (s.record rcn₂).progress ↔ (rcn₁ = rcn₂ ∨ rcn₁ ∈ s.progress) := by
-  simp [record, Set.insert]
--/
-
-/-
-theorem record_apply_comm {s : State α} {rcn : ID} : 
-    (s.record rcn).apply c = (s.apply c).record rcn := by
-  cases_change c <;> simp [apply, record]
-
-theorem record_apply'_comm {s : State α} {rcn : ID} : 
-    (s.record rcn).apply' cs = (s.apply' cs).record rcn := by
-  induction cs generalizing s
-  case nil => rfl
-  case cons hi => simp [apply', record_apply_comm]; exact hi 
-
-theorem record_exec_comm {s : State α} {rcn₁ rcn₂ : ID} : 
-    (s.record rcn₁).exec rcn₂ = (s.exec rcn₂).record rcn₁ := by
-  simp [exec]
-  rw [←output_progress_agnostic (s₁ := s) (s₂ := record s rcn₁) (i := rcn₂)]
-  exact record_apply'_comm
--/
-
--- TODO: Is this being used?
-def record' [DecidableEq ID] (s : State α) (rcns : List ID) : State α := 
-  { s with progress := s.progress ∪ { i | i ∈ rcns } }
-
-theorem record'_perm_eq {s : State α} (h : rcns₁ ~ rcns₂) : s.record' rcns₁ = s.record' rcns₂ := by
-  simp [record', h.mem_iff]
-  
-theorem mem_record'_progress_iff (s : State α) (rcns : List ID) (i : ID) :
-    i ∈ (s.record' rcns).progress ↔ (i ∈ s.progress ∨ i ∈ rcns) := by
-  simp [record']
+  | intro (mem : s.rtr[.rcn][i] = some rcn) (triggers : rcn.TriggersOn (s.input i)) 
 
 structure NextTag (s : State α) (next : Time.Tag) : Prop where
   mem   : next ∈ s.scheduledTags
   bound : s.tag < next
   least : ∀ g ∈ s.scheduledTags, (s.tag < g) → (next ≤ g)    
 
-theorem NextTag.isLeast {s : State α} (n : NextTag s g) : 
-    IsLeast { g' ∈ s.scheduledTags | s.tag < g' } g where
-  left := ⟨n.mem, n.bound⟩
-  right := by simp [lowerBounds]; exact n.least
-  
-theorem NextTag.deterministic {s : State α} (n₁ : NextTag s g₁) (n₂ : NextTag s g₂) : g₁ = g₂ :=
-  n₁.isLeast.unique n₂.isLeast
+def Closed (s : State α) : Prop := 
+  s.progress = s.rtr[.rcn].ids
 
-end State
-end Execution 
+def Nontrivial (s : State α) : Prop :=
+  s.rtr[.rcn].Nonempty
+
+end Execution.State
