src/ReactorModel/Execution/Theorems/Grouped/Tail.lean
@@ -5,19 +5,20 @@ open ReactorType
 
 namespace Execution.Grouped
 
-variable [Indexable α]
-
-inductive Tail : State α → State α → Type
-  | none  : Tail s s
+inductive Tail [Indexable α] : State α → State α → Type
+  | none : Tail s s
   | some : (s₁ ↓ᵢ+ s₂) → Tail s₁ s₂
 
 namespace Tail
 
-theorem preserves_tag {s₁ : State α} (e : Tail s₁ s₂) : s₁.tag = s₂.tag := by
-  sorry
+theorem preserves_tag [Indexable α] {s₁ s₂ : State α} : (Tail s₁ s₂) → s₁.tag = s₂.tag
+  | none => rfl
+  | some e => e.preserves_tag
 
-theorem deterministic {s₁ s₂ : State α} (e₁ : Tail s s₁) (e₂ : Tail s s₂) 
-    (hp : s₁.progress = s₂.progress) : s₁ = s₂ := by
-  sorry
+theorem deterministic [Readable α] {s s₁ s₂ : State α} (hp : s₁.progress = s₂.progress) :
+    (Tail s s₁) → (Tail s s₂) → s₁ = s₂
+  | none, none                  => rfl
+  | some e₁, some e₂            => e₁.deterministic e₂ (e₁.preserves_tag ▸ e₂.preserves_tag) hp
+  | none, some e | some e, none => e.progress_ne (by simp [hp]) |>.elim 
 
 end Execution.Grouped.Tail
