src/ReactorModel/Execution/Theorems/Step/Skip.lean
@@ -1,4 +1,5 @@
 import ReactorModel.Execution.Basic
+import ReactorModel.Execution.Theorems.State
 
 open Classical ReactorType Execution State
 
@@ -6,10 +7,10 @@ namespace Execution.Step.Skip
 
 variable [Indexable α] {s₁ : State α}
 
-def rcn :                      (s₁ ↓ₛ s₂) → ID                   | .mk (rcn := rcn) .. => rcn
-theorem allows_rcn :       (e : s₁ ↓ₛ s₂) → Allows s₁ e.rcn      | .mk a _ => a
-theorem not_triggers_rcn : (e : s₁ ↓ₛ s₂) → ¬Triggers s₁ e.rcn   | .mk _ t => t
-theorem dst_eq :           (e : s₁ ↓ₛ s₂) → s₂ = s₁.record e.rcn | .mk .. => rfl
+def rcn :                      (s₁ ↓ₛ s₂) → ID                   | mk (rcn := rcn) .. => rcn
+theorem allows_rcn :       (e : s₁ ↓ₛ s₂) → Allows s₁ e.rcn      | mk a _ => a
+theorem not_triggers_rcn : (e : s₁ ↓ₛ s₂) → ¬Triggers s₁ e.rcn   | mk _ t => t
+theorem dst_eq :           (e : s₁ ↓ₛ s₂) → s₂ = s₁.record e.rcn | mk .. => rfl
 
 theorem preserves_tag (e : s₁ ↓ₛ s₂) : s₁.tag = s₂.tag := by
   simp [e.dst_eq, State.record_preserves_tag]
@@ -20,5 +21,8 @@ theorem equiv (e : s₁ ↓ₛ s₂) : s₁.rtr ≈ s₂.rtr := by
 
 theorem progress_eq (e : s₁ ↓ₛ s₂) : s₂.progress = s₁.progress.insert e.rcn := by 
   simp [e.dst_eq, State.record_progress_eq]
+
+theorem preserves_nontrivial {e : s₁ ↓ₛ s₂} (n : s₁.Nontrivial) : s₂.Nontrivial :=
+  n.equiv e.equiv
 
 end Execution.Step.Skip
